<?xml version="1.0"?>
<rdf:RDF
    xmlns:argushiigi="http://data.travellerrpg.com/ontology/argushiigi#"
    xmlns:rdf="http://www.w3.org/1999/02/22-rdf-syntax-ns#"
    xmlns:terms="http://purl.org/dc/terms/"
    xmlns:owl="http://www.w3.org/2002/07/owl#"
    xmlns:skos="http://www.w3.org/2004/02/skos/core#"
    xmlns:rdfs="http://www.w3.org/2000/01/rdf-schema#"
    xmlns:xsd="http://www.w3.org/2001/XMLSchema#"
    xmlns="http://data.travellerrpg.com/ontology/argushiigi#"
  xml:base="http://data.travellerrpg.com/ontology/argushiigi">
  <owl:Ontology rdf:about="">
    <owl:imports rdf:resource="http://www.w3.org/2004/02/skos/core"/>
    <rdfs:isDefinedBy rdf:resource="https://github.com/makhidkarun/Argushiigi/wiki/Display-Ontology"/>
    <rdfs:comment xml:lang="en">The Argushiigi ontology allows annotations on other classes and properties that allow them to be organised and displayed in a human-readable form.</rdfs:comment>
    <rdfs:label rdf:datatype="http://www.w3.org/2001/XMLSchema#string"
    >Argushiigi</rdfs:label>
    <owl:imports rdf:resource="http://purl.org/dc/terms/"/>
    <terms:license rdf:resource="http://creativecommons.org/licenses/by/3.0/"/>
    <terms:creator rdf:resource="https://github.com/charvolant"/>
  </owl:Ontology>
  <owl:Class rdf:ID="Pattern">
    <rdfs:comment xml:lang="en">A formatting pattern.

Patterns are specific sequences of elements that can be combined to produce a textual representation of a resource. Individual properties are followed and rendered as required.</rdfs:comment>
    <rdfs:label xml:lang="en">Pattern</rdfs:label>
  </owl:Class>
  <owl:Class rdf:ID="SubPattern">
    <rdfs:comment xml:lang="en">Down the rabbit hole. A pattern derived from a reference to a property. The value of the property is used to format the sub-pattern. 

The format held by this pattern is the format applied to the value of the property.</rdfs:comment>
    <rdfs:subClassOf>
      <owl:Restriction>
        <owl:onClass>
          <owl:Class rdf:ID="Format"/>
        </owl:onClass>
        <owl:qualifiedCardinality rdf:datatype="http://www.w3.org/2001/XMLSchema#nonNegativeInteger"
        >1</owl:qualifiedCardinality>
        <owl:onProperty>
          <owl:AnnotationProperty rdf:ID="format">
            <skos:scopeNote xml:lang="en">Properties and classes may have a seperate labelFormat and valueFormat, so that statements can be properly modelled. If there are no specific label- or value- annotations then the format applies to the value.</skos:scopeNote>
            <rdf:type rdf:resource="http://www.w3.org/2002/07/owl#FunctionalProperty"/>
            <rdfs:label xml:lang="en">format</rdfs:label>
            <rdfs:range>
              <owl:Class rdf:about="#Format"/>
            </rdfs:range>
            <rdfs:comment xml:lang="en">Gives the format a resource or resource of this class uses.

Formats are generally associated with classes or properties. However, a resource may have its own format.</rdfs:comment>
            <rdf:type rdf:resource="http://www.w3.org/2002/07/owl#ObjectProperty"/>
          </owl:AnnotationProperty>
        </owl:onProperty>
      </owl:Restriction>
    </rdfs:subClassOf>
    <rdfs:label xml:lang="en">pattern</rdfs:label>
    <rdfs:subClassOf rdf:resource="#Pattern"/>
  </owl:Class>
  <owl:Class rdf:ID="Category">
    <rdfs:label xml:lang="en">Display Category</rdfs:label>
    <rdfs:comment xml:lang="en">A named category things to display.

Display categories can be organised into a hierarchy.</rdfs:comment>
  </owl:Class>
  <owl:Class rdf:about="#Format">
    <rdfs:comment xml:lang="en">A way of formatting a resource textually. 

Formats provide a mechanism for displaying "value-like" resources. A class with a format is expected to be displayed in-line, rather than as a link.

A format contains a sequence of literals and patterns, references to specific properties and ways of formatting them that can be used to extract information and format it.  All patterns in a sequence must match for the format to be used, otherwise the next pattern is tried.</rdfs:comment>
    <rdfs:label xml:lang="en">Format</rdfs:label>
  </owl:Class>
  <owl:ObjectProperty rdf:ID="property">
    <rdfs:range rdf:resource="http://www.w3.org/1999/02/22-rdf-syntax-ns#Property"/>
    <rdfs:label xml:lang="en">from property</rdfs:label>
    <rdfs:comment xml:lang="en">Gives the property that this pattern draws data from.</rdfs:comment>
    <rdfs:domain rdf:resource="#Pattern"/>
    <rdf:type rdf:resource="http://www.w3.org/2002/07/owl#FunctionalProperty"/>
  </owl:ObjectProperty>
  <owl:ObjectProperty rdf:ID="sortProperty">
    <rdfs:range rdf:resource="http://www.w3.org/1999/02/22-rdf-syntax-ns#Property"/>
    <rdfs:label xml:lang="en">sort property</rdfs:label>
    <rdfs:comment xml:lang="en">The property to use to order  information in a category</rdfs:comment>
    <rdfs:domain rdf:resource="#Category"/>
  </owl:ObjectProperty>
  <owl:ObjectProperty rdf:ID="pattern">
    <rdfs:comment xml:lang="en">The sequence of pattern elements to use when attempting a format. Each element is tried in turn and the format accepted or rejected, based on whether the element is optional or not.</rdfs:comment>
    <rdfs:domain rdf:resource="#Format"/>
    <rdfs:label xml:lang="en">pattern</rdfs:label>
    <rdfs:range rdf:resource="http://www.w3.org/1999/02/22-rdf-syntax-ns#Seq"/>
  </owl:ObjectProperty>
  <owl:DatatypeProperty rdf:ID="implementationFormat">
    <rdfs:domain rdf:resource="#Pattern"/>
    <rdfs:comment xml:lang="en">A format description specific to a particular (computer) language or system's conventions.</rdfs:comment>
  </owl:DatatypeProperty>
  <owl:DatatypeProperty rdf:ID="multiple">
    <rdfs:comment xml:lang="en">Indicates that there are multiple statements of this form. If set to true, then a list of statements, separated by commas is generated</rdfs:comment>
    <rdfs:domain rdf:resource="#Pattern"/>
    <rdfs:range rdf:resource="http://www.w3.org/2001/XMLSchema#boolean"/>
    <rdfs:label xml:lang="en">multiple</rdfs:label>
    <skos:scopeNote xml:lang="en">If absent, a pattern is assumed to be a singleton.</skos:scopeNote>
  </owl:DatatypeProperty>
  <owl:DatatypeProperty rdf:ID="eHex">
    <rdfs:range rdf:resource="http://www.w3.org/2001/XMLSchema#boolean"/>
    <rdfs:seeAlso rdf:resource="http://data.travellerrpg.com/publication/Traveller5Core"/>
    <rdfs:subPropertyOf rdf:resource="#implementationFormat"/>
    <rdfs:comment xml:lang="en">Indicates that a value should be expressed as Traveller-style eHex.

eHex values are extended hexadecimal, with the following values

decimal ehex

0-9 0-9
10-17 A-H
x I (omitted)
18-22 J-N
x O (omitted)
23-33 P-Z

Additional codes are

unknown X
special Y
ulitmate Z

</rdfs:comment>
    <rdfs:label xml:lang="en">eHex</rdfs:label>
  </owl:DatatypeProperty>
  <owl:DatatypeProperty rdf:ID="required">
    <rdfs:comment xml:lang="en">Indicates that a pattern element is required.</rdfs:comment>
    <rdfs:domain rdf:resource="#Pattern"/>
    <rdfs:range rdf:resource="http://www.w3.org/2001/XMLSchema#boolean"/>
    <skos:scopeNote xml:lang="en">If absent, a pattern is assumed to be required.</skos:scopeNote>
    <rdfs:label xml:lang="en">required</rdfs:label>
  </owl:DatatypeProperty>
  <owl:TransitiveProperty rdf:ID="parentCategory">
    <rdfs:domain rdf:resource="#Category"/>
    <rdfs:range rdf:resource="#Category"/>
    <rdfs:comment xml:lang="en">The parent category of a sub-category.

This property can be used to build embedded hierarchies of categories.</rdfs:comment>
    <rdf:type rdf:resource="http://www.w3.org/2002/07/owl#FunctionalProperty"/>
    <rdf:type rdf:resource="http://www.w3.org/2002/07/owl#ObjectProperty"/>
  </owl:TransitiveProperty>
  <owl:FunctionalProperty rdf:ID="literal">
    <rdfs:domain rdf:resource="#Pattern"/>
    <rdfs:comment xml:lang="en">A literal value to format.

The literal can be any literal value, not just text. If a format is specified then the format will be used to format the literal.</rdfs:comment>
    <rdfs:label xml:lang="en">literal</rdfs:label>
    <rdf:type rdf:resource="http://www.w3.org/2002/07/owl#DatatypeProperty"/>
  </owl:FunctionalProperty>
  <owl:FunctionalProperty rdf:ID="language">
    <rdfs:domain>
      <owl:Class>
        <owl:unionOf rdf:parseType="Collection">
          <owl:Class rdf:about="#Format"/>
          <owl:Class rdf:about="#Pattern"/>
        </owl:unionOf>
      </owl:Class>
    </rdfs:domain>
    <rdfs:range rdf:resource="http://www.w3.org/2001/XMLSchema#language"/>
    <rdfs:comment xml:lang="en">Associates a format or pattern with a specific language.

If not specified, the format or pattern applies to any language.</rdfs:comment>
    <rdfs:label xml:lang="en">language</rdfs:label>
    <rdf:type rdf:resource="http://www.w3.org/2002/07/owl#DatatypeProperty"/>
  </owl:FunctionalProperty>
  <owl:FunctionalProperty rdf:ID="javaFormat">
    <rdfs:subPropertyOf rdf:resource="#implementationFormat"/>
    <rdfs:label xml:lang="en">java format</rdfs:label>
    <rdfs:comment xml:lang="en">The format to use when displaying this property in Java.

This uses java.text.MessageFormat syntax to define the property, with the value of the property as argument 0, the name of the property as argument 1 and the name of the subject of the statement as argument 2.</rdfs:comment>
    <rdf:type rdf:resource="http://www.w3.org/2002/07/owl#DatatypeProperty"/>
  </owl:FunctionalProperty>
  <owl:AnnotationProperty rdf:ID="valueFormat">
    <rdfs:label xml:lang="en">value format</rdfs:label>
    <rdfs:subPropertyOf rdf:resource="#format"/>
    <rdfs:comment xml:lang="en">The format to use for a value</rdfs:comment>
  </owl:AnnotationProperty>
  <rdf:Description rdf:about="http://www.w3.org/2004/02/skos/core#hiddenLabel">
    <argushiigi:category>
      <argushiigi:Category rdf:about="http://data.travellerrpg.com/argushiigi/name">
        <rdfs:comment xml:lang="en">The name category, used to locate labels and titles that can be used to name an object.</rdfs:comment>
        <rdfs:label xml:lang="en">Name</rdfs:label>
        <argushiigi:parentCategory>
          <argushiigi:Category rdf:about="http://data.travellerrpg.com/argushiigi/top">
            <rdfs:label xml:lang="en">Top</rdfs:label>
            <rdfs:comment xml:lang="en">The top-level category. Used as a catch-all for uncategorised elements.</rdfs:comment>
            <argushiigi:priority rdf:datatype="http://www.w3.org/2001/XMLSchema#integer"
            >1000</argushiigi:priority>
          </argushiigi:Category>
        </argushiigi:parentCategory>
        <argushiigi:priority rdf:datatype="http://www.w3.org/2001/XMLSchema#integer"
        >10</argushiigi:priority>
      </argushiigi:Category>
    </argushiigi:category>
    <argushiigi:priority rdf:datatype="http://www.w3.org/2001/XMLSchema#integer"
    >100</argushiigi:priority>
  </rdf:Description>
  <owl:AnnotationProperty rdf:about="http://www.w3.org/2004/02/skos/core#historyNote"/>
  <owl:AnnotationProperty rdf:ID="priority">
    <rdfs:label xml:lang="en">display priority</rdfs:label>
    <rdfs:comment xml:lang="en">The priority of this item in any list of items to be displayed.</rdfs:comment>
    <skos:historyNote xml:lang="en">This was originally intended to be a system for defining partial orders. Too hard.</skos:historyNote>
    <rdfs:range rdf:resource="http://www.w3.org/2001/XMLSchema#integer"/>
  </owl:AnnotationProperty>
  <argushiigi:Category rdf:about="http://data.travellerrpg.com/argushiigi/reference">
    <rdfs:comment xml:lang="en">The category containing references to a resource</rdfs:comment>
    <rdfs:label xml:lang="en">Reference</rdfs:label>
    <argushiigi:parentCategory rdf:resource="http://data.travellerrpg.com/argushiigi/top"/>
    <argushiigi:priority rdf:datatype="http://www.w3.org/2001/XMLSchema#integer"
    >900</argushiigi:priority>
  </argushiigi:Category>
  <owl:AnnotationProperty rdf:ID="category">
    <rdfs:range rdf:resource="#Category"/>
    <rdfs:comment xml:lang="en">Places an entity into a category. Display categories can be used to annotate classes, properties and individuals. Classes and properties inherit categories from super-entities, using the closest super-entity with the lowest priority.</rdfs:comment>
    <rdfs:label xml:lang="en">category</rdfs:label>
  </owl:AnnotationProperty>
  <rdf:Description rdf:about="http://www.w3.org/2004/02/skos/core#altLabel">
    <argushiigi:category rdf:resource="http://data.travellerrpg.com/argushiigi/name"/>
    <argushiigi:priority rdf:datatype="http://www.w3.org/2001/XMLSchema#integer"
    >50</argushiigi:priority>
  </rdf:Description>
  <rdf:Description rdf:about="http://www.w3.org/2004/02/skos/core#prefLabel">
    <argushiigi:category rdf:resource="http://data.travellerrpg.com/argushiigi/name"/>
    <argushiigi:priority rdf:datatype="http://www.w3.org/2001/XMLSchema#integer"
    >10</argushiigi:priority>
  </rdf:Description>
  <rdf:Description rdf:about="http://www.w3.org/2000/01/rdf-schema#label">
    <argushiigi:priority rdf:datatype="http://www.w3.org/2001/XMLSchema#integer"
    >30</argushiigi:priority>
  </rdf:Description>
  <owl:AnnotationProperty rdf:ID="labelFormat">
    <rdfs:comment xml:lang="en">The format to use for a label</rdfs:comment>
    <rdfs:subPropertyOf rdf:resource="#format"/>
    <rdfs:label xml:lang="en">label format</rdfs:label>
  </owl:AnnotationProperty>
</rdf:RDF>

<!-- Created with TopBraid -->
