<?xml version="1.0"?>


<!DOCTYPE rdf:RDF [
    <!ENTITY terms "http://purl.org/dc/terms/" >
    <!ENTITY skos "http://xmlns.com/foaf/0.1/" >
    <!ENTITY owl "http://www.w3.org/2002/07/owl#" >
    <!ENTITY xsd "http://www.w3.org/2001/XMLSchema#" >
    <!ENTITY core "http://www.w3.org/2004/02/skos/core#" >
    <!ENTITY rdfs "http://www.w3.org/2000/01/rdf-schema#" >
    <!ENTITY rpg "http://data.travellerrpg.com/ontology/rpg#" >
    <!ENTITY rdf "http://www.w3.org/1999/02/22-rdf-syntax-ns#" >
]>


<rdf:RDF xmlns="http://data.travellerrpg.com/ontology/rpg#"
     xml:base="http://data.travellerrpg.com/ontology/rpg"
     xmlns:rdfs="http://www.w3.org/2000/01/rdf-schema#"
     xmlns:terms="http://purl.org/dc/terms/"
     xmlns:owl="http://www.w3.org/2002/07/owl#"
     xmlns:xsd="http://www.w3.org/2001/XMLSchema#"
     xmlns:rdf="http://www.w3.org/1999/02/22-rdf-syntax-ns#"
     xmlns:core="http://www.w3.org/2004/02/skos/core#"
     xmlns:skos="http://xmlns.com/foaf/0.1/"
     xmlns:rpg="http://data.travellerrpg.com/ontology/rpg#">
    <owl:Ontology rdf:about="http://data.travellerrpg.com/ontology/rpg">
        <core:scopeNote xml:lang="en">RPGs represent imaginary situations.

Data available on the semantic web represent a wide variety of resources, from the wholely imaginary to the completely real.

This ontology imports SKOS for knowledge descriptions and FOAF for player information. Otherwise, it keeps the real world at a distance, so that difficulties with software confusing a cyberpunk description of London and the real London are kept to a minimum.</core:scopeNote>
        <rdfs:comment xml:lang="en">The RPG ontology contains abstract descriptions of common RPG concepts, such as Characters, Skills, NPCs etc. A specigic RPG will specialise these concepts to fit the RPG.
</rdfs:comment>
        <rdfs:seeAlso rdf:resource="http://www.travellerrpg.com/CotI/Discuss/showthread.php?t=30041"/>
        <owl:imports rdf:resource="http://www.w3.org/2004/02/skos/core"/>
        <owl:imports rdf:resource="http://xmlns.com/foaf/0.1/"/>
        <terms:creator rdf:resource="https://github.com/charvolant"/>
    </owl:Ontology>
    


    <!-- 
    ///////////////////////////////////////////////////////////////////////////////////////
    //
    // Object Properties
    //
    ///////////////////////////////////////////////////////////////////////////////////////
     -->

    


    <!-- http://data.travellerrpg.com/ontology/rpg#hasAttribute -->

    <owl:ObjectProperty rdf:about="&rpg;hasAttribute">
        <rdfs:label xml:lang="en">has attribute</rdfs:label>
        <rdfs:comment xml:lang="en">Gives the attributes that describe an actor</rdfs:comment>
        <rdfs:range rdf:resource="&rpg;Attribute"/>
        <rdfs:domain rdf:resource="&rpg;GameEntity"/>
        <rdfs:subPropertyOf rdf:resource="&rpg;hasFeature"/>
    </owl:ObjectProperty>
    


    <!-- http://data.travellerrpg.com/ontology/rpg#hasFaculty -->

    <owl:ObjectProperty rdf:about="&rpg;hasFaculty">
        <rdfs:comment xml:lang="en">Indicates that an actor has a specific faculty available</rdfs:comment>
        <rdfs:range rdf:resource="&rpg;FacultyLevel"/>
        <rdfs:domain rdf:resource="&rpg;GameEntity"/>
        <rdfs:subPropertyOf rdf:resource="&rpg;hasFeature"/>
    </owl:ObjectProperty>
    


    <!-- http://data.travellerrpg.com/ontology/rpg#hasFeature -->

    <owl:ObjectProperty rdf:about="&rpg;hasFeature">
        <rdfs:label xml:lang="en">has feature</rdfs:label>
        <rdfs:comment xml:lang="en">Indicates that a character possesses a certain feature.</rdfs:comment>
        <rdfs:range rdf:resource="&rpg;Feature"/>
        <rdfs:domain rdf:resource="&rpg;GameEntity"/>
    </owl:ObjectProperty>
    


    <!-- http://data.travellerrpg.com/ontology/rpg#hasMass -->

    <owl:ObjectProperty rdf:about="&rpg;hasMass">
        <rdfs:label xml:lang="en">mass</rdfs:label>
        <rdfs:comment xml:lang="en">Gives the basic mass of a game item.</rdfs:comment>
        <rdfs:range rdf:resource="&rpg;Mass"/>
        <rdfs:subPropertyOf rdf:resource="&rpg;hasAttribute"/>
    </owl:ObjectProperty>
    


    <!-- http://data.travellerrpg.com/ontology/rpg#hasSense -->

    <owl:ObjectProperty rdf:about="&rpg;hasSense">
        <rdfs:label xml:lang="en">has sense</rdfs:label>
        <rdfs:comment xml:lang="en">Indicates that an actor has a specific sense available</rdfs:comment>
        <rdfs:domain rdf:resource="&rpg;GameEntity"/>
        <rdfs:range rdf:resource="&rpg;SenseLevel"/>
        <rdfs:subPropertyOf rdf:resource="&rpg;hasFeature"/>
    </owl:ObjectProperty>
    


    <!-- http://data.travellerrpg.com/ontology/rpg#hasSkill -->

    <owl:ObjectProperty rdf:about="&rpg;hasSkill">
        <rdfs:label xml:lang="en">has skill</rdfs:label>
        <rdfs:comment xml:lang="en">Indicates that an actor has a level of a specific skill</rdfs:comment>
        <rdfs:domain rdf:resource="&rpg;GameEntity"/>
        <rdfs:range rdf:resource="&rpg;SkillLevel"/>
        <rdfs:subPropertyOf rdf:resource="&rpg;hasFeature"/>
    </owl:ObjectProperty>
    


    <!-- http://data.travellerrpg.com/ontology/rpg#isInSetting -->

    <owl:ObjectProperty rdf:about="&rpg;isInSetting">
        <rdf:type rdf:resource="&owl;TransitiveProperty"/>
        <rdfs:label xml:lang="en">is in setting</rdfs:label>
        <rdfs:comment xml:lang="en">Indicates that a setting takes place in the context of a larger setting.</rdfs:comment>
        <rdfs:range rdf:resource="&rpg;Setting"/>
        <rdfs:domain rdf:resource="&rpg;Setting"/>
    </owl:ObjectProperty>
    


    <!-- http://data.travellerrpg.com/ontology/rpg#isInState -->

    <owl:ObjectProperty rdf:about="&rpg;isInState">
        <rdfs:label xml:lang="en">is in state</rdfs:label>
        <rdfs:comment xml:lang="en">Indicates that a game item is currently in a particular state</rdfs:comment>
        <rdfs:domain rdf:resource="&rpg;GameEntity"/>
        <rdfs:range rdf:resource="&rpg;State"/>
    </owl:ObjectProperty>
    


    <!-- http://data.travellerrpg.com/ontology/rpg#isPortrayedBy -->

    <owl:ObjectProperty rdf:about="&rpg;isPortrayedBy">
        <rdfs:label xml:lang="en">is portrayed by</rdfs:label>
        <rdfs:comment xml:lang="en">Indicates that a character is portrayed by a specific participant.</rdfs:comment>
        <rdfs:domain rdf:resource="&rpg;Character"/>
        <rdfs:range rdf:resource="&rpg;Participant"/>
        <owl:inverseOf rdf:resource="&rpg;portrays"/>
    </owl:ObjectProperty>
    


    <!-- http://data.travellerrpg.com/ontology/rpg#portrays -->

    <owl:ObjectProperty rdf:about="&rpg;portrays">
        <rdfs:label xml:lang="en">portrays</rdfs:label>
        <rdfs:comment xml:lang="en">A participant portrays a character, speaking for the characters actions and controling the character&apos;s decsiions.</rdfs:comment>
        <rdfs:range rdf:resource="&rpg;Character"/>
        <rdfs:domain rdf:resource="&rpg;Participant"/>
    </owl:ObjectProperty>
    


    <!-- http://data.travellerrpg.com/ontology/rpg#template -->

    <owl:ObjectProperty rdf:about="&rpg;template">
        <rdf:type rdf:resource="&owl;TransitiveProperty"/>
        <rdfs:label xml:lang="en">template</rdfs:label>
        <rdfs:comment xml:lang="en">Indicates that the subject uses the object as a template.</rdfs:comment>
        <rdfs:domain rdf:resource="&rpg;GameEntity"/>
        <rdfs:range rdf:resource="&rpg;GameEntity"/>
        <rdfs:range rdf:resource="&rpg;Template"/>
    </owl:ObjectProperty>
    


    <!-- 
    ///////////////////////////////////////////////////////////////////////////////////////
    //
    // Classes
    //
    ///////////////////////////////////////////////////////////////////////////////////////
     -->

    


    <!-- http://data.travellerrpg.com/ontology/rpg#Actor -->

    <owl:Class rdf:about="&rpg;Actor">
        <rdfs:label xml:lang="en">Actor</rdfs:label>
        <rdfs:subClassOf rdf:resource="&rpg;GameEntity"/>
        <rdfs:comment xml:lang="en">Something that can be interacted with within the game. 

Actors can be modelled within the game to various degrees of fidelity. For example, a player character may be more detailed than an animal that the character encounters.</rdfs:comment>
    </owl:Class>
    


    <!-- http://data.travellerrpg.com/ontology/rpg#Adventure -->

    <owl:Class rdf:about="&rpg;Adventure">
        <rdfs:label xml:lang="en">Adventure</rdfs:label>
        <rdfs:subClassOf rdf:resource="&rpg;Setting"/>
        <rdfs:comment xml:lang="en">A story-level setting for a game, usually with a clear beginning, middle and end.</rdfs:comment>
    </owl:Class>
    


    <!-- http://data.travellerrpg.com/ontology/rpg#Attribute -->

    <owl:Class rdf:about="&rpg;Attribute">
        <rdfs:label xml:lang="en">Attribute</rdfs:label>
        <rdfs:subClassOf rdf:resource="&rpg;Feature"/>
        <rdfs:comment xml:lang="en">A descriptive attribute of a character or item.</rdfs:comment>
        <core:scopeNote xml:lang="en">Attributes are generally fixed things about a character or things which change very slowly. 

Attributes are generally central to the game system and are descibed via subclassing for a specific RPG, rather than by referencing individuals.</core:scopeNote>
        <core:example xml:lang="en">Examples are strength, size, education, as well as sex, hair colour, etc.</core:example>
    </owl:Class>
    


    <!-- http://data.travellerrpg.com/ontology/rpg#Campaign -->

    <owl:Class rdf:about="&rpg;Campaign">
        <rdfs:label xml:lang="en">Campaign</rdfs:label>
        <rdfs:subClassOf rdf:resource="&rpg;Setting"/>
        <rdfs:comment xml:lang="en">A series of events and adventures featuring a continuing set of chracters and settings.</rdfs:comment>
    </owl:Class>
    


    <!-- http://data.travellerrpg.com/ontology/rpg#Character -->

    <owl:Class rdf:about="&rpg;Character">
        <rdfs:label xml:lang="en">Character</rdfs:label>
        <rdfs:subClassOf rdf:resource="&rpg;Actor"/>
        <rdfs:comment xml:lang="en">An RPG representation of a person or similar within-game creature capable of making its own decsions. </rdfs:comment>
        <core:scopeNote xml:lang="en">Characters are usually modelled as something that could be controlled by a player, even if the character is not.</core:scopeNote>
    </owl:Class>
    


    <!-- http://data.travellerrpg.com/ontology/rpg#Extra -->

    <owl:Class rdf:about="&rpg;Extra">
        <rdfs:label xml:lang="en">Extra</rdfs:label>
        <rdfs:subClassOf rdf:resource="&rpg;Actor"/>
        <rdfs:comment xml:lang="en">A game actor modelled to a low level of detail.</rdfs:comment>
        <core:example xml:lang="en">A wandering monster, a background soldier or a bureaucrat.</core:example>
    </owl:Class>
    


    <!-- http://data.travellerrpg.com/ontology/rpg#Faculty -->

    <owl:Class rdf:about="&rpg;Faculty">
        <rdfs:label xml:lang="en">Faculty</rdfs:label>
        <rdfs:subClassOf rdf:resource="&core;Concept"/>
        <rdfs:comment xml:lang="en">A type of inherent ability or power.</rdfs:comment>
    </owl:Class>
    


    <!-- http://data.travellerrpg.com/ontology/rpg#FacultyLevel -->

    <owl:Class rdf:about="&rpg;FacultyLevel">
        <rdfs:label xml:lang="en">Faculty Level</rdfs:label>
        <rdfs:subClassOf rdf:resource="&rpg;Feature"/>
        <rdfs:comment xml:lang="en">The level of power for an inherent ability or power.</rdfs:comment>
    </owl:Class>
    


    <!-- http://data.travellerrpg.com/ontology/rpg#Feature -->

    <owl:Class rdf:about="&rpg;Feature">
        <rdfs:label xml:lang="en">Feature</rdfs:label>
        <rdfs:comment xml:lang="en">Something that describes a character or an item: a characteristic, a skill, an ability, etc.</rdfs:comment>
    </owl:Class>
    


    <!-- http://data.travellerrpg.com/ontology/rpg#GameEntity -->

    <owl:Class rdf:about="&rpg;GameEntity">
        <rdfs:label xml:lang="en">Game Entity</rdfs:label>
        <rdfs:comment xml:lang="en">Something that exists with the role playing game.</rdfs:comment>
    </owl:Class>
    


    <!-- http://data.travellerrpg.com/ontology/rpg#GameMaster -->

    <owl:Class rdf:about="&rpg;GameMaster">
        <rdfs:label xml:lang="en">Game Master</rdfs:label>
        <rdfs:subClassOf rdf:resource="&rpg;Participant"/>
        <rdfs:comment xml:lang="en">The participant responsible for creating and managing the situation that forms the role playing game.

The game master has, in theory if not in practice, complete knowledge of the game world. The game master is also generally responsible for refereeing decsicions within the game.</rdfs:comment>
    </owl:Class>
    


    <!-- http://data.travellerrpg.com/ontology/rpg#Item -->

    <owl:Class rdf:about="&rpg;Item">
        <rdfs:label xml:lang="en">Item</rdfs:label>
        <rdfs:subClassOf rdf:resource="&rpg;GameEntity"/>
        <rdfs:comment xml:lang="en">An object within the game that can be used or owned by an actor.</rdfs:comment>
    </owl:Class>
    


    <!-- http://data.travellerrpg.com/ontology/rpg#Mass -->

    <owl:Class rdf:about="&rpg;Mass">
        <rdfs:label xml:lang="en">Mass</rdfs:label>
        <rdfs:subClassOf rdf:resource="&rpg;Attribute"/>
        <rdfs:comment xml:lang="en">The basic mass of an item or character.

Generally, this means the most convienient defintiion for role-playing purposes. A character&apos;s mass is their mass in ordingary clothing, without additional items such as armour. A weapon&apos;s mass is generally its mass with a full load of ammunition.

Depending on setting, mass and weight may be two different things. eg. in Zero-G an item has no weight but still has mass. For purely single-world games, the terms are interchanable.</rdfs:comment>
        <core:altLabel xml:lang="en">Weight</core:altLabel>
    </owl:Class>
    


    <!-- http://data.travellerrpg.com/ontology/rpg#Milieau -->

    <owl:Class rdf:about="&rpg;Milieau">
        <rdfs:label xml:lang="en">Milieau</rdfs:label>
        <rdfs:subClassOf rdf:resource="&rpg;Setting"/>
        <rdfs:comment xml:lang="en">The large-scale setting of a campaign or an adventure. An outline of the world or universe that the game takes place in.</rdfs:comment>
    </owl:Class>
    


    <!-- http://data.travellerrpg.com/ontology/rpg#NonPlayerCharacter -->

    <owl:Class rdf:about="&rpg;NonPlayerCharacter">
        <rdfs:label>Non-Player Character</rdfs:label>
        <rdfs:subClassOf rdf:resource="&rpg;Character"/>
        <rdfs:subClassOf>
            <owl:Restriction>
                <owl:onProperty rdf:resource="&rpg;isPortrayedBy"/>
                <owl:allValuesFrom rdf:resource="&rpg;GameMaster"/>
            </owl:Restriction>
        </rdfs:subClassOf>
        <core:prefLabel>NPC</core:prefLabel>
        <rdfs:comment xml:lang="en">A character controlled by a game master or some other agent, such as a software program.</rdfs:comment>
    </owl:Class>
    


    <!-- http://data.travellerrpg.com/ontology/rpg#Participant -->

    <owl:Class rdf:about="&rpg;Participant">
        <rdfs:label xml:lang="en">Participant</rdfs:label>
        <rdfs:subClassOf rdf:resource="&skos;Agent"/>
        <rdfs:comment xml:lang="en">A participant in a role playing game.

Participants are usually a singular Person. However, groups are also possible.</rdfs:comment>
    </owl:Class>
    


    <!-- http://data.travellerrpg.com/ontology/rpg#Player -->

    <owl:Class rdf:about="&rpg;Player">
        <rdfs:label xml:lang="en">Player</rdfs:label>
        <rdfs:subClassOf rdf:resource="&rpg;Participant"/>
        <rdfs:comment xml:lang="en">A player in a role playing game &quot;plays&quot; a one or more characters within the game.

The player has partial knowledge of the game situation.</rdfs:comment>
    </owl:Class>
    


    <!-- http://data.travellerrpg.com/ontology/rpg#PlayerCharacter -->

    <owl:Class rdf:about="&rpg;PlayerCharacter">
        <rdfs:label xml:lang="en">Player Character</rdfs:label>
        <rdfs:subClassOf rdf:resource="&rpg;Character"/>
        <rdfs:subClassOf>
            <owl:Restriction>
                <owl:onProperty rdf:resource="&rpg;isPortrayedBy"/>
                <owl:allValuesFrom rdf:resource="&rpg;Player"/>
            </owl:Restriction>
        </rdfs:subClassOf>
        <rdfs:comment xml:lang="en">A character directly controlled by a player.</rdfs:comment>
    </owl:Class>
    


    <!-- http://data.travellerrpg.com/ontology/rpg#Rules -->

    <owl:Class rdf:about="&rpg;Rules">
        <rdfs:label>Rules</rdfs:label>
        <rdfs:subClassOf rdf:resource="&core;ConceptScheme"/>
        <rdfs:subClassOf rdf:resource="&skos;Document"/>
        <rdfs:comment xml:lang="en">A specific set of RPG rules.

Rules can be used to define which sets of rules are compatible with characters, settings, etc.</rdfs:comment>
        <rdfs:seeAlso rdf:resource="&rpg;SourceBook"/>
    </owl:Class>
    


    <!-- http://data.travellerrpg.com/ontology/rpg#Sense -->

    <owl:Class rdf:about="&rpg;Sense">
        <rdfs:label xml:lang="en">Sense</rdfs:label>
        <rdfs:subClassOf rdf:resource="&core;Concept"/>
        <rdfs:comment xml:lang="en">The ability to sense a specific form of phenomenon.</rdfs:comment>
        <core:example xml:lang="en">Visible light, sound, infravision (infrared light), magic.</core:example>
    </owl:Class>
    


    <!-- http://data.travellerrpg.com/ontology/rpg#SenseLevel -->

    <owl:Class rdf:about="&rpg;SenseLevel">
        <rdfs:label xml:lang="en">Sense Level</rdfs:label>
        <rdfs:subClassOf rdf:resource="&rpg;Feature"/>
        <rdfs:comment xml:lang="en">The ability to sense something at a particular level.

The mehanics of how sense work form part of a specific RPGs mechanics.</rdfs:comment>
    </owl:Class>
    


    <!-- http://data.travellerrpg.com/ontology/rpg#Setting -->

    <owl:Class rdf:about="&rpg;Setting">
        <rdfs:label xml:lang="en">Setting</rdfs:label>
        <rdfs:comment xml:lang="en">A setting is the stage that an RPG is played on. Settings range in scale from entire universes to the bar in which an adventure takes place. A setting may refer to a location, a time period, a social mileau or any combination.</rdfs:comment>
    </owl:Class>
    


    <!-- http://data.travellerrpg.com/ontology/rpg#Skill -->

    <owl:Class rdf:about="&rpg;Skill">
        <rdfs:label xml:lang="en">Skill</rdfs:label>
        <rdfs:subClassOf rdf:resource="&core;Concept"/>
        <rdfs:comment xml:lang="en">A type of skill. Skills are learned abilities that can be improved by a character exercising the skill or undergoing training.</rdfs:comment>
    </owl:Class>
    


    <!-- http://data.travellerrpg.com/ontology/rpg#SkillLevel -->

    <owl:Class rdf:about="&rpg;SkillLevel">
        <rdfs:label xml:lang="en">Skill Level</rdfs:label>
        <rdfs:subClassOf rdf:resource="&rpg;Feature"/>
        <rdfs:comment xml:lang="en">A level of ability in a specific skill.

The way that skill levels are represented are specific to a game system.</rdfs:comment>
    </owl:Class>
    


    <!-- http://data.travellerrpg.com/ontology/rpg#SourceBook -->

    <owl:Class rdf:about="&rpg;SourceBook">
        <rdfs:label xml:lang="en">Source Book</rdfs:label>
        <rdfs:subClassOf rdf:resource="&skos;Document"/>
        <rdfs:comment xml:lang="en">Additional information about a setting.

Conceptually, rules define the mechanics of a game and a source book defines the environment to which the rules apply. In practice, an RPG usually consists of a combined set of rules and setting.</rdfs:comment>
        <rdfs:seeAlso rdf:resource="&rpg;Rules"/>
    </owl:Class>
    


    <!-- http://data.travellerrpg.com/ontology/rpg#State -->

    <owl:Class rdf:about="&rpg;State">
        <rdfs:label xml:lang="en">State</rdfs:label>
        <rdfs:comment xml:lang="en">A changable status for something in a game.</rdfs:comment>
        <core:example xml:lang="en">Examples are things like health statistics, unconciosness, asleep for characters and oiut of ammunition for a gun.</core:example>
        <core:scopeNote xml:lang="en">States are generally strongly connected to the mechanics of an RPG and are generally directly modelled for a specific game.</core:scopeNote>
    </owl:Class>
    


    <!-- http://data.travellerrpg.com/ontology/rpg#Template -->

    <owl:Class rdf:about="&rpg;Template">
        <rdfs:label xml:lang="en">Tempate</rdfs:label>
        <rdfs:comment xml:lang="en">Something that is a template represents an abstract class-like description of a game item. A template can be used to describe a generic instance of an item. Individual items can inherit from the template and override speicifc elements.
</rdfs:comment>
        <core:scopeNote xml:lang="en">Templates can inherit from other templates. The rules on how inheritance is managed are game-specific.</core:scopeNote>
        <core:scopeNote xml:lang="en">The template class is usually added to other entities to indicate that the entity is for use as a template.</core:scopeNote>
    </owl:Class>
</rdf:RDF>



<!-- Generated by the OWL API (version 3.4.2) http://owlapi.sourceforge.net -->

